wip

code/streaming/Hacl.Streaming.HMAC.fst
@@ -18,16 +18,7 @@ open Hacl.Streaming.Interface
 
 #set-options "--max_fuel 0 --max_ifuel 0 --z3rlimit 100"
 
-/// We find ourselves in the same situation as with the most recent iteration of
-/// Blake2: the key here is variable length, and the copy function would be
-/// really hard to write if the source and destination had possibly different
-/// key lengths (what to do? reallocate?), so we fix the key length *in the
-/// index* so that we can statically enforce that the lengths match. This means
-/// that a client of the streaming HMAC interface cannot copy from one state to
-/// another if they key lengths differ.
-type index = i:impl & l:UInt32.t { Spec.Agile.HMAC.keysized (alg_of_impl i) (UInt32.v l) }
-
-let stateful_agile_hash_state: Hacl.Streaming.Interface.stateful index =
+let stateful_agile_hash_state: Hacl.Streaming.Interface.stateful Hacl.Streaming.HMAC.Definitions.index =
   Hacl.Streaming.Interface.Stateful
     (fun i -> state (dfst i))
     (fun #i h s -> footprint #(dfst i) s h)
@@ -45,75 +36,7 @@ let stateful_agile_hash_state: Hacl.Streaming.Interface.stateful index =
     (fun i -> free #(dfst i))
     (fun i -> copy #(dfst i))
 
-// Stateful key definition, keeps its length at runtime
-
-let state (i: index) = (b:B.buffer uint8 { B.len b == dsnd i }) & B.pointer UInt32.t
-
-let footprint (#i: index) h (s: state i): GTot B.loc =
-  let k, l = s in
-  (if dsnd i = 0ul then B.loc_none else B.loc_addr_of_buffer k) `B.loc_union` B.loc_addr_of_buffer l
-
-let invariant (#i: index) h (s: state i): Type0 =
-  let k, l = s in
-  B.len k == B.deref h l /\ B.live h l /\ B.deref h l == dsnd i /\ (
-  dsnd i <> 0ul ==>
-    B.(loc_disjoint (loc_addr_of_buffer k) (loc_addr_of_buffer l)) /\ B.live h k)
-
-let t (i: index) =
-  s:S.seq uint8 { S.length s == UInt32.v (dsnd i) }
-
-let v (i: index) h (s: state i) =
-  let k, l = s in
-  (B.as_seq h k <: t i)
-
-inline_for_extraction noextract
-let stateful_runtime_key: stateful index =
-  Stateful
-    (* s *) (fun i -> state i)
-    (* footprint *) footprint
-    (* freeable *) (fun #i h (k, l) -> (if dsnd i <> 0ul then B.freeable k else True) /\ B.freeable l)
-    (* invariant *) (fun #i h s -> invariant #i h s)
-    (* t *) (fun i -> t i)
-    (* v *) v
-    (* invariant_loc_in_footprint *) (fun #_ h s -> let k, l = s in ())
-    (* frame_invariant *) (fun (#i: index) l (s: state i) (h0: HS.mem) (h1: HS.mem) ->
-      let k, l = s in
-      if dsnd i = 0ul then begin
-        let v0 = v i h0 s in
-        let v1 = v i h1 s in
-        assert (v0 `S.equal` v1)
-      end;
-      ()
-    )
-    (* frame_freeable *) (fun #_ l s h0 h1 -> ())
-    (* alloca *) (fun i ->
-      let l = dsnd i in
-      if l = 0ul then
-        let k = B.null in
-        let l = B.alloca l 1ul in
-        let h = ST.get () in
-        k, l
-      else
-        B.alloca (Lib.IntTypes.u8 0) l, B.alloca l 1ul
-    )
-    (* create_in *) (fun i r -> (if dsnd i = 0ul then B.null else B.malloc r Lib.IntTypes.(u8 0) (dsnd i)), B.malloc r (dsnd i) 1ul)
-    (* free *) (fun _ (k, l) -> if !*l <> 0ul then B.free k; B.free l)
-    (* copy *) (fun i s_src s_dst ->
-      let k_src, l_src = s_src in
-      let k_dst, l_dst = s_dst in
-      let l_src = !*l_src in
-      let l_dst = !*l_dst in
-      assert (l_src == l_dst);
-      let h0 = ST.get () in
-      if l_src <> 0ul then
-        B.blit k_src 0ul k_dst 0ul l_src;
-      let h1 = ST.get () in
-      assert (S.equal (B.as_seq h1 k_dst) (B.as_seq h1 k_src)))
-
-inline_for_extraction noextract
-let alg (i: index) = alg_of_impl (dfst i)
-
-#set-options "--max_fuel 0 --max_ifuel 0 --z3rlimit 100"
+open Hacl.Streaming.HMAC.Definitions
 
 let index_of_state (i: G.erased index) (s: Hacl.Agile.Hash.state (dfst i)) (k: state i): Stack index
   (requires (fun h0 -> Hacl.Agile.Hash.invariant s h0 /\ invariant h0 k))
@@ -177,7 +100,7 @@ let hmac: block index =
     (* spec_is_incremental *) (fun i k input l ->
       Spec.HMAC.Incremental.hmac_is_hmac_incremental (alg i) k input)
     (* index_of_state *) index_of_state
-    (* init *) (fun i k buf s -> admit ())
+    (* init *) (fun i k buf s -> init i k buf s)
     (* update_multi *) (fun i s prevlen blocks len ->
       Hacl.Agile.Hash.update_multi s prevlen blocks len
     )
