code/streaming/Hacl.Streaming.HMAC.Definitions.fst
@@ -1,0 +1,25 @@
+module Hacl.Streaming.HMAC.Definitions
+
+/// Helper definitions with an interface so as to friend Spec.Agile.HMAC
+
+open FStar.HyperStack.ST
+open LowStar.BufferOps
+
+module HS = FStar.HyperStack
+module ST = FStar.HyperStack.ST
+module B = LowStar.Buffer
+module M = LowStar.Modifies
+module G = FStar.Ghost
+module S = FStar.Seq
+module D = Hacl.Hash.Definitions
+
+open Hacl.Agile.Hash
+open Hacl.Streaming.Interface
+
+#set-options "--max_fuel 0 --max_ifuel 0 --z3rlimit 100"
+
+friend Spec.Agile.HMAC
+friend Spec.Incremental.HMAC
+
+let init k buf s =
+  admit ()
