code/streaming/Hacl.Streaming.HMAC.Definitions.fsti
@@ -1,0 +1,128 @@
+module Hacl.Streaming.HMAC.Definitions
+
+/// Helper definitions with an interface so as to friend Spec.Agile.HMAC
+
+open FStar.HyperStack.ST
+open LowStar.BufferOps
+
+module HS = FStar.HyperStack
+module ST = FStar.HyperStack.ST
+module B = LowStar.Buffer
+module M = LowStar.Modifies
+module G = FStar.Ghost
+module S = FStar.Seq
+module D = Hacl.Hash.Definitions
+
+open Hacl.Agile.Hash
+open Hacl.Streaming.Interface
+
+#set-options "--max_fuel 0 --max_ifuel 0 --z3rlimit 100"
+
+/// We find ourselves in the same situation as with the most recent iteration of
+/// Blake2: the key here is variable length, and the copy function would be
+/// really hard to write if the source and destination had possibly different
+/// key lengths (what to do? reallocate?), so we fix the key length *in the
+/// index* so that we can statically enforce that the lengths match. This means
+/// that a client of the streaming HMAC interface cannot copy from one state to
+/// another if they key lengths differ.
+type index = i:impl & l:UInt32.t { Spec.Agile.HMAC.keysized (alg_of_impl i) (UInt32.v l) }
+
+///////////////////////////////////////////////////////
+// Stateful key definition, keeps its length at runtime
+///////////////////////////////////////////////////////
+
+let state (i: index) = (b:B.buffer uint8 { B.len b == dsnd i }) & B.pointer UInt32.t
+
+let footprint (#i: index) h (s: state i): GTot B.loc =
+  let k, l = s in
+  (if dsnd i = 0ul then B.loc_none else B.loc_addr_of_buffer k) `B.loc_union` B.loc_addr_of_buffer l
+
+let invariant (#i: index) h (s: state i): Type0 =
+  let k, l = s in
+  B.len k == B.deref h l /\ B.live h l /\ B.deref h l == dsnd i /\ (
+  dsnd i <> 0ul ==>
+    B.(loc_disjoint (loc_addr_of_buffer k) (loc_addr_of_buffer l)) /\ B.live h k)
+
+let t (i: index) =
+  s:S.seq uint8 { S.length s == UInt32.v (dsnd i) }
+
+let v (i: index) h (s: state i) =
+  let k, l = s in
+  (B.as_seq h k <: t i)
+
+let freeable #i h (s: state i) =
+  let k, l = s in
+  (if dsnd i <> 0ul then B.freeable k else True) /\ B.freeable l
+
+inline_for_extraction noextract
+let stateful_runtime_key: stateful index =
+  Stateful
+    (* s *) (fun i -> state i)
+    (* footprint *) footprint
+    (* freeable *) (fun #i h s -> freeable h s)
+    (* invariant *) (fun #i h s -> invariant h s)
+    (* t *) (fun i -> t i)
+    (* v *) v
+    (* invariant_loc_in_footprint *) (fun #_ h s -> let k, l = s in ())
+    (* frame_invariant *) (fun (#i: index) l (s: state i) (h0: HS.mem) (h1: HS.mem) ->
+      let k, l = s in
+      if dsnd i = 0ul then begin
+        let v0 = v i h0 s in
+        let v1 = v i h1 s in
+        assert (v0 `S.equal` v1)
+      end;
+      ()
+    )
+    (* frame_freeable *) (fun #_ l s h0 h1 -> ())
+    (* alloca *) (fun i ->
+      let l = dsnd i in
+      if l = 0ul then
+        let k = B.null in
+        let l = B.alloca l 1ul in
+        let h = ST.get () in
+        k, l
+      else
+        B.alloca (Lib.IntTypes.u8 0) l, B.alloca l 1ul
+    )
+    (* create_in *) (fun i r -> (if dsnd i = 0ul then B.null else B.malloc r Lib.IntTypes.(u8 0) (dsnd i)), B.malloc r (dsnd i) 1ul)
+    (* free *) (fun _ (k, l) -> if !*l <> 0ul then B.free k; B.free l)
+    (* copy *) (fun i s_src s_dst ->
+      let k_src, l_src = s_src in
+      let k_dst, l_dst = s_dst in
+      let l_src = !*l_src in
+      let l_dst = !*l_dst in
+      assert (l_src == l_dst);
+      let h0 = ST.get () in
+      if l_src <> 0ul then
+        B.blit k_src 0ul k_dst 0ul l_src;
+      let h1 = ST.get () in
+      assert (S.equal (B.as_seq h1 k_dst) (B.as_seq h1 k_src)))
+
+/////////////////////////////////////////////////
+// Helper functions that need to be under an fsti
+/////////////////////////////////////////////////
+
+inline_for_extraction noextract
+let alg (i: index) = alg_of_impl (dfst i)
+
+val init: (i:G.erased index -> (
+    let i = G.reveal i in
+    k: state i ->
+    buf_: B.buffer uint8 { B.length buf_ = UInt32.v (D.block_len (alg i)) } ->
+    s: Hacl.Agile.Hash.state (dfst i) -> Stack unit
+    (requires fun h0 ->
+      invariant #i h0 k /\
+      B.live h0 buf_ /\
+      Hacl.Agile.Hash.invariant #(dfst i) s h0 /\
+      B.loc_disjoint (footprint h0 k) (Hacl.Agile.Hash.footprint s h0) /\
+      B.loc_disjoint (footprint h0 k) (B.loc_buffer buf_) /\
+      B.loc_disjoint (B.loc_buffer buf_) (Hacl.Agile.Hash.footprint s h0))
+    (ensures fun h0 _ h1 ->
+      invariant h1 k /\
+      (freeable h0 k ==> freeable h1 k) /\
+      Hacl.Agile.Hash.invariant s h1 /\
+      Hacl.Agile.Hash.repr s h1 == Spec.HMAC.Incremental.init (alg i) (v i h0 k) /\
+      S.equal (S.slice (B.as_seq h1 buf_) 0 (UInt32.v (D.block_len (alg i)))) (Spec.HMAC.Incremental.init_input (alg i) (v i h0 k)) /\
+      B.(modifies (loc_union (Hacl.Agile.Hash.footprint s h0) (loc_buffer buf_)) h0 h1) /\
+      Hacl.Agile.Hash.footprint s h0 == Hacl.Agile.Hash.footprint s h1 /\
+      (Hacl.Agile.Hash.freeable h0 s ==> Hacl.Agile.Hash.freeable h1 s))))
