providers/evercrypt/fst/EverCrypt.Hash.Incremental.fst
@@ -140,7 +140,7 @@ let evercrypt_hash : block Hash.alg =
         assert (S.equal input1 input);
         Spec.Hash.Incremental.hash_is_hash_incremental' a input ())
 
-    EverCrypt.Hash.alg_of_state
+    (fun a s _ -> EverCrypt.Hash.alg_of_state a s)
     (fun i _ _ -> EverCrypt.Hash.init #i)
     (fun i s prevlen blocks len -> EverCrypt.Hash.update_multi #i s prevlen blocks len)
     (fun i s prevlen last last_len ->
